SetRelation.v
@@ -1,0 +1,254 @@
+Require Export
+  Coq.Sets.Ensembles.
+
+Require Import
+  Coq.Program.Tactics.
+
+Section SetRelation.
+
+Variable A : Type.
+Variable B : Type.
+
+Record SetRel := mkSetRel {
+  relEns : Ensemble (A * B);
+  _      : forall a b b',
+             In _ relEns (a, b)  ->
+             In _ relEns (a, b') -> b = b'
+}.
+
+Program Definition Empty : SetRel := mkSetRel (Empty_set (A * B)) _.
+Obligation 1. inversion H. Qed.
+
+Program Definition Insert
+        (a : A) (b : B) (r : SetRel)
+        (H : forall b' : B, ~ In _ (relEns r) (a, b')) : SetRel :=
+  mkSetRel (Add _ (relEns r) (a, b)) _.
+Obligation 1.
+  destruct r; simpl in *.
+  inversion H0; inversion H1; clear H0 H1;
+  try (inversion H2; clear H2);
+  try (inversion H4; clear H4);
+  subst; firstorder.
+Qed.
+
+Program Definition Remove (a : A) (r : SetRel) : SetRel :=
+  mkSetRel (Setminus _ (relEns r) (fun p => fst p = a)) _.
+Obligation 1.
+  destruct r; simpl in *.
+  inversion H; inversion H0; clear H H0;
+  subst; firstorder.
+Qed.
+
+Lemma Remove_spec : forall a r r',
+  Remove a r = r' -> forall b' : B, ~ In _ (relEns r') (a, b').
+Proof.
+  unfold Remove, relEns, Setminus, In.
+  intros; subst.
+  firstorder.
+Qed.
+
+Program Definition Update (a : A) (b : B) (r : SetRel) : SetRel :=
+  Insert a b (Remove a r) _.
+Obligation 1.
+  unfold Remove, relEns, Setminus, In.
+  intros; subst.
+  firstorder.
+Qed.
+
+Program Definition Move (a a' : A) (r : SetRel) : SetRel :=
+  mkSetRel (fun p => IF fst p = a'
+                     then relEns r (a, snd p)
+                     else relEns (Remove a r) p) _.
+Obligation 1.
+  unfold Remove, relEns.
+  destruct r; simpl in *.
+  inversion H; inversion H0; clear H H0;
+  firstorder.
+Qed.
+
+Program Definition Filter (P : A * B -> Prop) (r : SetRel) : SetRel :=
+  mkSetRel (fun p => P p /\ relEns r p) _.
+Obligation 1. destruct r; simpl in *; firstorder. Qed.
+
+Program Definition Map (f : A * B -> B) (r : SetRel) : SetRel :=
+  mkSetRel (fun p : A * B =>
+              exists b : B,
+                In _ (relEns r) (fst p, b) /\
+                In _ (Singleton _ (fst p, f (fst p, b))) p) _.
+Obligation 1.
+  destruct r; simpl in *;
+  firstorder; simpl in *.
+  specialize (e _ _ _ H H0); subst.
+  inversion H1; inversion H2; clear H1 H2.
+  reflexivity.
+Qed.
+
+Program Definition Modify (a : A) (f : B -> B) (r : SetRel) : SetRel :=
+  mkSetRel (fun p : A * B =>
+              IF fst p = a
+              then exists b : B,
+                In _ (relEns r) (fst p, b) /\
+                In _ (Singleton _ (f b)) (snd p)
+              else In _ (relEns r) p) _.
+Obligation 1.
+  destruct r; simpl in *;
+  firstorder; simpl in *.
+  specialize (e _ _ _ H1 H3); subst.
+  inversion H2; inversion H4; clear H2 H4.
+  reflexivity.
+Qed.
+
+Definition RemoveIf (P : A * B -> Prop) (r : SetRel) : SetRel :=
+  Filter (fun p => ~ P p) r.
+
+Definition All (P : A * B -> Prop) (r : SetRel) : Prop :=
+  forall p, In _ (relEns r) p -> P p.
+
+Definition Any (P : A * B -> Prop) (r : SetRel) : Prop :=
+  exists p, In _ (relEns r) p -> P p.
+
+Program Definition Define (P : A -> Prop) (b : B) (r : SetRel) : SetRel :=
+  mkSetRel (fun p => IF P (fst p) then snd p = b else relEns r p) _.
+Obligation 1.
+  destruct r; simpl in *.
+  unfold In in *; simpl in *.
+  firstorder.
+  subst.
+  reflexivity.
+Qed.
+
+Program Definition Transfer (P : A -> option A) (r r' : SetRel) : SetRel :=
+  mkSetRel (fun p => forall a,
+              IF P a = Some (fst p)
+              then relEns r (a, snd p)
+              else relEns r' p) _.
+Obligation 1.
+  destruct r, r'; simpl in *.
+  unfold In in *; simpl in *.
+  specialize (H a).
+  specialize (H0 a).
+  destruct H, H0;
+  destruct (P a);
+  destruct H, H0;
+  firstorder.
+Qed.
+
+Definition Lookup (a : A) (b : B) (r : SetRel) := In _ (relEns r) (a, b).
+
+Lemma All_Lookup : forall P r, All P r -> forall a b, Lookup a b r -> P (a, b).
+Proof.
+  unfold All, Lookup; intros.
+  firstorder.
+Qed.
+
+Lemma Lookup_Remove : forall a b a' r,
+  Lookup a b (Remove a' r) -> a <> a' /\ Lookup a b r.
+Proof. firstorder. Qed.
+
+Lemma Lookup_Remove_impl : forall a b a' r,
+  Lookup a b r -> a <> a' -> Lookup a b (Remove a' r).
+Proof. firstorder. Qed.
+
+Lemma Lookup_Update : forall a b a' b' r,
+  Lookup a b (Update a' b' r)
+    -> IF a = a' then b = b' else Lookup a b r.
+Proof.
+  intros.
+  inversion H; clear H.
+    firstorder.
+  inversion H0; clear H0.
+  firstorder.
+Qed.
+
+Lemma Lookup_Move : forall a b a' a'' r,
+  Lookup a b (Move a' a'' r)
+    -> IF a = a''
+       then Lookup a' b r
+       else a <> a' /\ Lookup a b r.
+Proof. firstorder. Qed.
+
+Lemma Lookup_Map : forall a b f r,
+  Lookup a b (Map f r)
+    -> exists b', f (a, b') = b /\ Lookup a b' r.
+Proof.
+  intros.
+  inversion H; clear H.
+    firstorder.
+  inversion H0; clear H0.
+  firstorder.
+Qed.
+
+Lemma Lookup_Modify : forall a b a' f r,
+  Lookup a b (Modify a' f r)
+    -> IF a = a'
+       then exists b', f b' = b /\ Lookup a b' r
+       else Lookup a b r.
+Proof.
+  intros.
+  inversion H; clear H;
+  destruct H0.
+    destruct H0.
+    destruct H0.
+    inversion H1; simpl in *; subst.
+    left; split; trivial.
+    exists x.
+    split; trivial.
+  right; split; trivial.
+Qed.
+
+Definition Member (a : A) (r : SetRel) := exists b, In _ (relEns r) (a, b).
+
+Lemma Member_Remove (addr : A) mem :
+  forall addr', Member addr' mem
+    -> addr' <> addr
+    -> Member addr' (Remove addr mem).
+Proof. firstorder. Qed.
+
+Lemma Member_Lookup : forall a r, Member a r -> exists b, Lookup a b r.
+Proof. firstorder. Qed.
+
+Lemma Lookup_Member : forall a b r, Lookup a b r -> Member a r.
+Proof. firstorder. Qed.
+
+Definition FindA (P : A -> Prop) (b : B) (r : SetRel) :=
+  forall a, Lookup a b r /\ P a.
+
+Definition FindB (P : B -> Prop) (a : A) (r : SetRel) :=
+  forall b, Lookup a b r /\ P b.
+
+End SetRelation.
+
+Arguments mkSetRel : default implicits.
+Arguments relEns : default implicits.
+Arguments Empty : default implicits.
+Arguments Insert : default implicits.
+Arguments Remove : default implicits.
+Arguments Update : default implicits.
+Arguments Modify : default implicits.
+Arguments Move : default implicits.
+Arguments Filter : default implicits.
+Arguments Map : default implicits.
+Arguments RemoveIf : default implicits.
+Arguments All : default implicits.
+Arguments Any : default implicits.
+Arguments Define : default implicits.
+Arguments Transfer : default implicits.
+Arguments Lookup : default implicits.
+Arguments Member : default implicits.
+Arguments FindA : default implicits.
+Arguments FindB : default implicits.
+
+Ltac teardown :=
+  repeat
+    match goal with
+    | [ H : Lookup _ _ (Modify _ _ _) |- _ ] => apply Lookup_Modify in H
+    | [ H : Lookup _ _ (Update _ _ _) |- _ ] => apply Lookup_Update in H
+    | [ H : Lookup _ _ (Move _ _ _)   |- _ ] => apply Lookup_Move in H
+    | [ H : Lookup _ _ (Map _ _)      |- _ ] => apply Lookup_Map in H
+    | [ H : Lookup _ _ (Remove _ _)   |- _ ] => apply Lookup_Remove in H
+
+    | [ H : IF _ then _ else _ |- _ ] => destruct H
+    | [ H : _ /\ _             |- _ ] => destruct H
+    | [ H : exists _, _        |- _ ] => destruct H
+
+    end; try tauto.
